\documentclass{article}
\usepackage[cp1251]{inputenc}
\usepackage[russian]{babel}
\usepackage{amsmath,amsfonts,amssymb,latexsym,amsbsy}
\usepackage{epic, eepic}
\begin{document}

\textbf{1.}
$$
\left\{
\begin{array}{l}
2x_1+x_2+x_3=5\\
x_1-2x_2+3x_3=5\\
7x_1+x_2-x_3=10\\
\end{array}\right.
$$
������� ������� ��������� � ���� ����������� �������:

$	\left(
\begin{array}{ccc|c}
2&-3&1&-1\\
5&2&-1&0\\
2&-3&2&3\\
\end{array}\right)  $=
$	\left(
\begin{array}{ccc|c}
1&-1.5&0.5&-0.5\\
5&2&-1&0\\
2&-3&2&3\\
\end{array}\right)  $=
$	\left(
\begin{array}{ccc|c}
1&-1.5&0.5&-0.5\\
0&9.5&-3.5&2.5\\
0&0&1&4\\
\end{array}\right)  $=

����� ������������� �������������� �������:

$=	\left(
\begin{array}{ccc|c}
1&-1.5&0.5&-0.5\\
0&1&-7/19&9/15\\
0&0&1&4\\
\end{array}\right)  $=
$	\left(
\begin{array}{ccc|c}
1&0&-1/19&-2/19\\
0&1&-7/19&5/19\\
\end{array}\right)  $=
$	\left(
\begin{array}{ccc|c}
1&0&0&2/19\\
0&1&0&33/19\\
0&0&1&4\\
\end{array}\right). $
\begin{flushright}
\textbf{�����:} $	x_1=2/19, x_2=33/19, x_3=4.$
\end{flushright}



\textbf{2.} �������� ������������ �����:
$$5x^2+6xy+5y^2-16x-16=0$$ � ������������� ����.

$a_{11}=5$
$a_{12}=3$ 
$a_{22}=2$

$
\begin{array}{|cc|}
5-\lambda&3\\
3&2-\lambda\\
\end{array}  =0$

$(5-\lambda)(2-\lambda)-9=0$

$(\lambda)^2-7\lambda+10-9=0$

$(\lambda)^2-7\lambda+1=0$

$D=49-1=48$

$\lambda_1=\dfrac{7-\sqrt{48}}{2}=\dfrac{0.1}{2}=0.05$

$\lambda_1=\dfrac{7+\sqrt{48}}{2}=\dfrac{13.9}{2}=6.95$

$0.05x^2+6.95x^2-16=0$

$0.05x^2+6.95x^2=16$

$\dfrac{0.05x^2}{16}+\dfrac{6.95x^2}{16}=1$

$\dfrac{x^2}{320}+\dfrac{x^2}{2.3}=1.$

\textbf{3.}��������� ��������� ������� �������:

1)
$$\lim_{x\to1}{\dfrac{(x^2+3x+2)^2}{x^3+2x^2-x^2}}=\dfrac{(1+3+2)^2}{1+2-1}=\dfrac{36}{2}=18.$$

2) ��������� ������� ��������.
$$\lim_{x\to0}{\dfrac{3x^2-5x}{\sin{3x}}}=\Bigl(\dfrac{0}{0}\Bigr)=\dfrac{6x+5}{3\cos{3x}}=\dfrac{5}{3}.$$

3) ��������� ������� ��������.
$$\lim_{x\to0}{\dfrac{6^{2x}-7^{-2x}}{\sin{3x}-2x}}=\Bigl(\dfrac{0}{0}\Bigr)=\lim_{x\to0}\dfrac{2x6^{2x-1}+2x7^{-2x-1}}{3\cos{3x}-2}=\dfrac{0}{1}=0.$$

4) ��������� ������� ��������.
$$\lim_{x\to-1}{\dfrac{x^3+1}{\sin{(x+1)}}}=\Bigl(\dfrac{0}{0}\Bigr)=\lim_{x\to-1}\dfrac{3x^2}{\cos{(x+1)}}=\dfrac{1}{1}=1.$$

5)
$$\lim_{x\to1}{\Bigl(\dfrac{2x-1}{x}\Bigr)^{\dfrac{1}{\sqrt[3]{x}-2}}=(1^1)=1}.$$

\textbf{4.} ��������� ��������� �����������:

1) $$y=\dfrac{x^4-8x^2}{2(x^2-4)} $$

��������� ������� ����������� ��������:
$$y'=\dfrac{(x^4-8x^2)'2(x^2-4)-(x^4-8x^2)2(x^2-4)'}{(2(x^2-4))^2}= $$
$$=\dfrac{2(4x^3-16x)(x^2-4)-2(x^4-8x^2)2x}{4(x^2-4)^2}=
\dfrac{2x(x^2-4)^2-(x^4-8x^2)x}{(x^2-4)^2}= $$
$$=\dfrac{2x(x^2-4)^2}{(x^2-4)^2}-\dfrac{(x^4-8x^2)x}{(x^2-4)^2}= $$
$$=2x-\dfrac{(x^2-8)x^3}{(x^2-4)^2}=2x-\dfrac{x^5-8x^3}{x^4-8x^2+16}$$
�������� ����� ����� �����.
$$=2x-x+\dfrac{16}{x^4-8x^2+16}=x+\Bigl(\dfrac{4}{x^2-4}\Bigr)^2.$$

2) $$y=\dfrac{2x-1}{4}\sqrt{2+x-x^2}+\dfrac{9}{8}\cdot\arcsin{\dfrac{2x-1}{3}} $$
$$y'=(\dfrac{1}{2}\sqrt{2+x-x^2}+\dfrac{(2x-1)(1-2x)}{8\sqrt{2+x-x^2}})+\dfrac{9}{8}\cdot\dfrac{\dfrac{2}{3}}{\sqrt{1-(\dfrac{2x-1}{3})^2}}= $$
$$=(\dfrac{1}{2}\sqrt{2+x-x^2}+\dfrac{(2x-1)(1-2x)}{8\sqrt{2+x-x^2}})+\dfrac{3}{4}\cdot\dfrac{3}{\sqrt{-4x^2+4x+8}}= $$
$$=\dfrac{1}{2}\sqrt{2+x-x^2}+\dfrac{(2x-1)(1-2x)}{8\sqrt{2+x-x^2}}+\dfrac{9}{8\sqrt{2+x-x^2}}= $$
$$=\dfrac{1}{2}\sqrt{2+x-x^2}+\dfrac{(2x-1)(1-2x)+9}{8\sqrt{2+x-x^2}}= $$
$$=\dfrac{1}{2}\sqrt{2+x-x^2}+\dfrac{8+4x-4x^2}{8\sqrt{2+x-x^2}}= $$
$$=\dfrac{1}{2}\sqrt{2+x-x^2}+\dfrac{4(2+x-x^2)}{8\sqrt{2+x-x^2}}= $$
$$=\sqrt{2+x-x^2}. $$

3)
$$y=\dfrac{1}{2}\ln{\dfrac{1+\sqrt{\th{x}}}{1+\sqrt{\th{x}}}-\arctg{\sqrt{\th{x}}}}= $$
$$=\dfrac{1}{2}\ln{1}-\arctg{\sqrt{\th{x}}}= $$
$$=0-\arctg{\sqrt{\th{x}}}= $$
$$y'=-\dfrac{1}{2(1+\th{x})\ch^2{x}\sqrt{\th{x}}}.$$

4)
$$y=\left(\sin{x} \right)^{5e^x}$$
$$\ln{y}=5e^x\cdot \ln{\left(\sin{x} \right)}$$
$$\dfrac{y'}{y}=\left(5e^x\cdot \ln{\left(\sin{x} \right)}\right)'=5e^x\cdot \ln{\left(\sin{x} \right)}+5e^x\cdot \dfrac{1}{\sin{x}}\cdot \cos{x} = $$
$$ = 5e^x\cdot \ln{\left(\sin{x} \right)}+5e^x\cdot \ctg{x} = 5e^{x}\cdot\left(\ln{\left(\sin{x} \right)}+\ctg{x}\right) $$
$$y'=y\cdot 5e^{x}\cdot\left(\ln{\left(\sin{x} \right)}+\operatorname{ctg}{x}\right) = \left(\sin{x} \right)^{5e^x}\cdot 5e^{x}\cdot\left(\ln{\left(\sin{x} \right)}+\operatorname{ctg}{x}\right) =$$
$$= 5e^{x}\cdot \left(\sin{x} \right)^{5e^x}\cdot \left(\ln{\left(\sin{x} \right)}+\ctg{x}\right).$$

5)
$$\begin{cases} 
x=\arcsin{\sqrt{t}}\\ 
y=\sqrt{1+\sqrt{t}}\end{cases} $$

$x'_{t}=(\arcsin{(\sqrt{t})})' = \frac{1}{\sqrt{1-t}}\cdot\dfrac{1}{2\sqrt{t}}$
$y'_{t}=(\sqrt{1+\sqrt{t}})' = \frac{1}{2\sqrt{1+\sqrt{t}}}\cdot\dfrac{1}{2\sqrt{t}} $
$$y'_{x}=\frac{y'_{t}}{x'_{t}} = (\frac{1}{\sqrt{1-t}}\cdot\dfrac{1}{2\sqrt{t}}):(\frac{1}{2\sqrt{1+\sqrt{t}}}\cdot\dfrac{1}{2\sqrt{t}})= $$
$$ = \frac{1}{\sqrt{1-t}}:\frac{1}{2\sqrt{1+\sqrt{t}}}=$$ $$=\frac{2\sqrt{1+\sqrt{t}}}{\sqrt{1-t}} = 2\sqrt{\frac{1}{1+\sqrt{t}}}.$$

\textbf{5.} ����������� ������� $y=\dfrac{x(12-x^2)}{8}$ � ��������� �� ������.

 \begin{enumerate}
 \item ������� ���������� �������:
 
 $D(f): x\in(-\infty;+\infty)$
 \item ������� �������� �������:
 
 $E(f): y\in(-\infty;+\infty)$
 \item ���� �������:
 
 $f(x)=0:$ 
 
 $x_1=-3.5;$ 
 
 $x_2=0;$ 
 
 $x_3=3.5 $ 
 \item ��������. 

$f(-x)=f(x) $ 
 ������� ��������
 \item �������������:
 
�.�.   $D(f): x\in(-\infty;+\infty)$
������� ����������
 	
����� ������� ��� 
 	
��������� ���
 \item ��������������:
 
 �.�. $E(f): y\in(-\infty;+\infty)$
 ������� ������������
 
 \item ����� ����������:
 
�.�. ��� $x< -2 f'(x)<0$,� $ -2<x<2 f'(x)>0 \Longrightarrow $ 

 $x=-2 - $ ����� ��������

��� $x>2 f'(x)<0$,� $ -2<x<2 f'(x)><0 \Longrightarrow $  
 $x=2 - $ ����� ���������
 
 \item ������������:
 
 �� ����������� ������ $\Longrightarrow$
 
 ������� ����������: $x\in(-2;2)$
 
 ������� �������: $x\in(-\infty;-2)\cup(2;\infty).$

 \end{enumerate}
 \unitlength=1cm
 \begin{picture}(12,4)(-6,-2)
 
 
 \thinlines
 \put(0,-2){\vector(0,1){4}}
 \put(-6,0){\vector(1,0){12}}
 \put(6.1,0.1){$x$}
 \put(0.1,2.1){$y$}
 \put(0.1,-0.4){$0$}
 \put(0.1,-1.4){$-1$}
 \put(0.1,1.1){$1$}
 \multiput(-6,-2)(1,0){13}{\dottedline{0.1}(0,0)(0,4)}
 \multiput(-6,-2)(0,1){5}{\dottedline{0.1}(0,0)(12,0)}
 \thicklines
  \path(-4,2)(-3.5,0)(-3,-1.125)(-2.5,-1.8)
(-2,-2)(-1.5,-1.828)(-1,-1.375)(-0.5,-0.734)
(0,0)(0.5,0.734)(1,1.375)(1.5,1.828)
(2,2)(2.5,1.8)(3,1.125)(3.5,0)(4,-2)
 \put(3.5,0.1){$3.5$}\put(3.5,0.0){\circle*{0.1}}
 \put(-3.5,0.1){$-3.5$}\put(-3.5,0.0){\circle*{0.1}}
 \end{picture} 

\textbf{6.}��������� ��������� (��������������, ������������, �������������):

1)$$\int (3x+4)e^{3x}dx = $$

����������� �� ������.
$$ = (3x+4)\cdot \frac{1}{3}e^{3x} - \int \frac{1}{3}e^{3x}\cdot 3dx = \frac{1}{3}\cdot (3x+4)e^{3x} - \int e^{3x}dx =$$

����������� �� ������.
$$ = \frac{1}{3}\cdot (3x+4)e^{3x} - \frac{1}{3}e^{3x} + C = \frac{1}{3}\cdot (3x+3)e^{3x} + C= (x+1)e^{3x} + C .$$

2)$$\int\limits_{-1}^0 \left(x^2+4x+3\right)\cos{x} dx = $$

$ = \left.\left(x^2+4x+3\right)\sin{x}\right|_{-1}^0 - \int\limits_{-1}^0 \sin{x}(2x+4)dx = $

$= \left(0^2+4\cdot 0+3\right)\sin{0} - \left((-1)^2+4\cdot (-1)+3\right)\sin{(-1)} - \int\limits_{-1}^0 \sin{x}(2x+4)dx = $

$= 3\cdot 0 - (1-4+3)\sin{(-1)} - \int\limits_{-1}^0 \sin{x}(2x+4)dx = - \int\limits_{-1}^0 \sin{x}(2x+4)dx =$

$= -\left( \left.(2x+4)\cdot \left( -\cos{x}\right)\right|_{-1}^0 - \int\limits_{-1}^0 \left(-\cos{x}\right)\cdot 2dx \right)=$

$ = -\left( (2\cdot 0+4)\cdot \left( -\cos{0}\right) - (2\cdot (-1)+4)\cdot \left( -\cos{(-1)}\right) + 2\int\limits_{-1}^0 \cos{x}dx \right)=$

$ = -\left( -4 + 2\cos{(-1)} + \left. 2\sin{x} \right|_{-1}^0\right) = -\left( -4 + 2\cos{1} + 2\sin{0} - 2\sin{(-1)} \right)=$

$= -\left( -4 + 2\cos{1} + 2\sin{1} \right) = 4 - 2\cos{1} - 2\sin{1}.$

3)
$$\int\limits_0^1 \dfrac{4\operatorname{arctg}{x}-x}{1+x^2} dx$$ 

���������� � ���� �������� ������:

$= 4\cdot \int\limits_0^1 \dfrac{\arctg{x}}{1+x^2} dx - \int\limits_0^1 \dfrac{x}{1+x^2} dx = $

������ ��� ���� ������������� ��������������� ���������:

$= 4\cdot \int\limits_0^1 \arctg{x}\cdot  d\left(\arctg{x}\right) - \dfrac{1}{2}\cdot \int\limits_0^1 \dfrac{d\left(1+x^2\right)}{1+x^2}  =$

$ = 4\cdot \left. \dfrac{1}{2}\arctg^{2}{x}\right|_0^1 - \dfrac{1}{2}\cdot \left.\ln{\left(1+x^2\right)}\right|_0^1 = $

$ = 2\operatorname{arctg}^{2}{1}-2\operatorname{arctg}^{2}{0} - \frac{1}{2}\cdot\left(\ln{\left(1+1^2\right)}-\ln{\left(1+0^2\right)}\right) =$

$ = 2\cdot \left(\dfrac{\pi}{4}\right)^2-2\cdot 0^2 - \dfrac{1}{2}\cdot\left(\ln{2}-\ln{1}\right) = \dfrac{\pi^2}{8} - \dfrac{1}{2}\cdot \ln{2} = \dfrac{\pi^2 - 4\cdot \ln{2}}{8}.$

4) $$\int \frac{x^3-17}{x^2-4x+3} dx = $$
������� ����� �����:
$$ = \int \left(x+4 + \frac{13x-29}{x^2-4x+3} \right)dx = \int (x+4)dx + \int \frac{13x-29}{(x-1)(x-3)}dx = $$
������� �������������� ������������� ���������� ����� � ���� ����� ������:
$$ = \int (x+4)dx + \int \left(\frac{8}{x-1} + \frac{5}{x-3}\right)dx =$$ $$=\frac{x^2}{2} + 4x + 8\ln{|x-1|} + 5\ln{|x-3|} + C. $$

5)$$\int\limits_0^{2\pi} \sin^{4}{x}\cos^{4}{x} dx$$ 

$=\int\limits_0^{2\pi}(\sin{x}\cdot\cos{x})^{4}dx = \int\limits_0^{2\pi}\left(\frac{\sin{2x}}{2}\right)^{4}dx = \frac{1}{16}\int\limits_0^{2\pi}\sin^{4}{2x}dx = $ 

$ = \frac{1}{16}\int\limits_0^{2\pi}\frac{1}{4}\cdot(1 - \cos{4x})^{2}dx = \frac{1}{64}\int\limits_0^{2\pi}(1 - 2\cos{4x} + \cos^{2}{4x})dx = $

$ = \frac{1}{64}\int\limits_0^{2\pi}\left(1 - 2\cos{4x} + \frac{1 + \cos{8x}}{2}\right)dx = \frac{1}{128}\int\limits_0^{2\pi}(2 - 4\cos{4x} + 1 + \cos{8x})dx = $

$= \frac{1}{128}\int\limits_0^{2\pi}(3 - 4\cos{4x} + \cos{8x})dx = \frac{1}{128}\left.\left(3x - \sin{4x} + \frac{\sin{8x}}{8}\right)\right|_{0}^{2\pi} = \frac{6\pi}{128} = \frac{3\pi}{64}.$

 
\textbf{7.} ��������� ������� �����, ������������ ��������� ������� $y=\dfrac{x}{1+\sqrt{x}}$ � $y=0,x=0$. ���������� ���������� ������.

 \unitlength=1cm
 \begin{picture}(12,6)(-1,-2)
 
 
 \thinlines
 \put(0,-2){\vector(0,1){6}}
 \put(-1,0){\vector(1,0){12}}
 \put(10.9,0.1){$x$}
 \put(0.1,3.9){$y$}
 \put(0.1,-0.4){$0$}
 \put(0.1,-1.4){$-1$}
 \put(0.1,1.1){$1$}
 \put(8,1.9){$y=\dfrac{x}{1+\sqrt{x}}$}
 \put(7.9,0.1){$x=0$}
 \put(0.1,2.9){$y=0$}
 
 
 \multiput(-1,-2)(1,0){13}{\dottedline{0.1}(0,0)(0,6)}
 \multiput(-1,-2)(0,1){7}{\dottedline{0.1}(0,0)(12,0)}
 \thicklines
  \path(0,0)(1,0.5)(2,0.83)(3,1.1)(4,1.33)(5,1.54)(9,2.25)(11,2.55)
 \put(1,0.1){$1$}\put(1,0.0){\circle*{0.1}}
 \put(-1,0.1){$-1$}\put(-1,0.0){\circle*{0.1}}
 \end{picture}
 ������� ������� ����� ���� ����� ����� (0;0), ��������, ������� ����� ����.

\textbf{8.} ��������� �������� $X$ ������ ������� �������������:

$\begin{array}{c|cccc}
\xi&1&3&6&8\\ \hline
\texttt{P}(\xi=x_i)&0.2&0.1&0.4&0.3\\
\end{array}$ ��������� �������������� �������������.����� ����������� ��������� �������: $P\{3\leq\xi\leq8\},P\{\xi>6\}. $

\textbf{9.} 50\% �������� � ����� - �������. 70\% ������� � 85\% ��������� ����� ������ � �����. � ����������� �������� ���-�� ���������� �����. ������ ����������� ����, ��� ����������� �������; ��������?

���� ������� �������:

$0.5\cdot0.7=0.35;$

���� ������� ���������:

$0.5\cdot0.85=0.425;$

����� � ��������:

$35+42=77;$

����������� ����, ��� ����� ����������� �������:

$\dfrac{35}{77}=0.45; $

����������� ����, ��� ����� ����������� ��������:

$\dfrac{42}{77}=0.54. $


\end{document}

















